$m = \lfloor \frac {An + B}{C} \rfloor$
$f(A, B, C, n) = \sum _{x = 0} ^ {n} \lfloor {Ax + B \over C}\rfloor nm - f(C, C - B - 1, A, m - 1)$
$g(A, B, C, n) = \sum _{x = 0} ^ {n}  i \lfloor \frac{Ax + B}{C} \rfloor = \frac {1}{2} \times [n(n + 1)m - f(C, C - B - 1, A, m - 1) - h(C, C - B - 1, A, m - 1)]$
$h(A, B, C, n) = \sum _{x = 0} ^ {n} \lfloor {Ax + B \over C}\rfloor ^ 2 = nm(m + 1) - 2g(C, C - B - 1, A, m - 1) - 2f(C, C - B - 1, A, m - 1) - f(A, B, C, n)$
分别考虑$A = 0$，$A \geq C$，$B \geq C$的边界
```
ll f(ll A,ll B,ll C,ll n)
{
    if (A == 0)
        return (n + 1) * (B / C);
    if (A < 0)
        return f(A + C * ((-A - 1) / C + 1), B, C, n) - n * (n + 1) / 2 * ((-A - 1) / C + 1);
    if (A >= C)
        return f(A % C, B, C, n) + n * (n + 1) / 2 * (A / C);
    if (B >= C)
        return f(A, B % C, C, n) + (n + 1) * (B / C);
    ll m = (A * n + B) / C;s
    return n * m - f(C, C - B - 1, A, m - 1);
}
```